PrimaryLogic/FirstOrder/Theorem.lean
@@ -3,9 +3,7 @@ import PrimaryLogic.FirstOrder.Axiom
 namespace PrimaryLogic
 namespace Proof
 variable {LF LP : Type} {L : Lang LF LP} {Γ : Set (Formula L)}
-
-private abbrev AX (Δ : Set (Formula L)) := Proof.axm (α := FOLAxioms L) (Γ := Δ)
-
+open FOL
 section propositional
 lemma refl_impl (x : Formula L) : Γ ⊢ x → x :=
   have p1 := AX Γ <| .h2 x (x → x) x
@@ -21,28 +19,29 @@ theorem deduction (Γ) (φ ψ : Formula L) :
   · intro p
     induction p with
     | asp x h =>
+      replace h : x ∈ insert φ Γ ∪ FOLTheory := h
+      rw [Set.mem_union, Set.mem_insert_iff, or_assoc] at h
       rcases h with (rfl | hi)
       · exact refl_impl x
       · exact (AX Γ (.h1 x φ)).mp (asp x hi)
-    | axm a => exact (AX Γ (.h1 (AxiomSchema.toFormula a) φ)).mp (AX Γ a)
     | @mp x y _ _ h1 h2 => exact ((AX Γ (.h2 φ x y)).mp h1).mp h2
   · intro p
     have : FOLProof (Γ.insert φ) (φ → ψ) :=
-      monotone (Set.subset_insert φ Γ) p
-    exact this.mp (asp φ (Set.mem_insert φ Γ))
+      mono (Set.subset_insert φ Γ) p
+    exact this.mp <| AS (Set.mem_insert φ Γ)
 
 lemma impl_trans {x y z : Formula L} :
     (Γ ⊢ x → y) -> (Γ ⊢ y → z) -> (Γ ⊢ x → z) := fun h g =>
   have h0 : (Γ.insert _).insert _ = (Γ.insert _).insert _ := Set.insert_comm' x (x → y → z) Γ
   have p1 := AX Γ (.h2 x y z)
   have p2 := (deduction Γ (x → y → z) ((x → y) → (x → z))).mpr p1
-  have p3 := monotone (Set.subset_insert (x → y → z) Γ) h
+  have p3 := mono (Set.subset_insert (x → y → z) Γ) h
   have p4 := mp p2 p3
   have p5 := (deduction _ x z).mpr p4
   have p6 := cast (by rw [h0]) p5
   have p7 := (deduction _ (x → y → z) z).mp p6
   have p8 := AX (Γ.insert x) (.h1 (y → z) x)
-  have p9 := monotone (Set.subset_insert x Γ) g
+  have p9 := mono (Set.subset_insert x Γ) g
   have p10 := mp p8 p9
   have p11 := mp p7 p10
   (deduction Γ x z).mp p11
@@ -64,9 +63,8 @@ lemma neg_impl (x y : Formula L) : (Γ ⊢ ¬x) -> (Γ ⊢ x → y) := fun h =>
 
 lemma intro_double_neg (x : Formula L) : Γ ⊢ x → ¬¬x :=
   let Δ := (Γ.insert x).insert (x → ⊥)
-  have as := asp (α := FOLAxioms L) (Γ := Δ)
-  have p1 := as (x → ⊥) <| by simp [Δ, Set.insert]
-  have p2 := as x <| by simp [Δ, Set.insert]
+  have p1 := AS (φ := x → ⊥) <| by simp only [Set.insert, Set.mem_setOf_eq, true_or]
+  have p2 := AS (φ := x) <| by simp only [Set.insert, Set.mem_setOf_eq, true_or, or_true]
   have p3 := p1.mp p2
   have p4 := deduction (Γ.insert x) (x → ⊥) ⊥
   have p5 := p4.mp p3
@@ -74,19 +72,18 @@ lemma intro_double_neg (x : Formula L) : Γ ⊢ x → ¬¬x :=
 
 lemma contrapositive (x y : Formula L) : Γ ⊢ (¬x → ¬y) → (y → x) :=
   let Δ := (Γ.insert ((x → ⊥) → (y → ⊥))).insert y
-  have as := asp (α := FOLAxioms L) (Γ := Δ.insert (x → ⊥))
-  have p1 := as ((x → ⊥) → (y → ⊥)) <| by simp [Δ, Set.insert]
-  have p2 := as y <| by simp [Δ, Set.insert]
-  have p3 := as (x → ⊥) <| by simp [Set.insert]
+  have p1 := AS (φ := (x → ⊥) → (y → ⊥)) <| by simp [Δ, Set.insert]
+  have p2 := AS (φ := y) <| by simp [Δ, Set.insert]
+  have p3 := AS (φ := x → ⊥) <| by simp [Set.insert]
   have p4 := p1.mp p3
   have p5 := p4.mp p2
   have p6 := (deduction Δ (x → ⊥) ⊥).mp p5
-  have p7 := Proof.axm (α := FOLAxioms L) (Γ := Δ) (.h3 x)
+  have p7 := AX Δ (.h3 x)
   have p8 := p7.mp p6
   have p9 := (deduction (Γ.insert ((x → ⊥) → (y → ⊥))) y x).mp p8
   (deduction Γ ((x → ⊥) → (y → ⊥)) (y → x)).mp p9
 
-lemma raa (x : Formula L) : (Γ ⊢ x) <-> Inconsistent (FOLAxioms L) (Γ.insert (¬x)) := by
+lemma raa (x : Formula L) : (Γ ⊢ x) <-> Inconsistent (Γ.insert (¬x) ∪ FOLTheory) := by
   unfold Inconsistent
   constructor
   · intro p
@@ -104,8 +101,17 @@ theorem gen_rule (φ : Formula L) (i : Idx) :
     (∀ g ∈ Γ, i ∉ g.fvar) -> (Γ ⊢ φ) -> (Γ ⊢ ∀i# φ) := by
   intro hg p
   induction p with
-  | asp ψ h => exact (AX Γ (.q3 i ψ (hg ψ h))).mp (asp ψ h)
-  | axm a => exact AX Γ (.gen i a)
+  | asp ψ h =>
+    rw [Set.mem_union] at h
+    rcases h with h1 | h2
+    · exact (AX Γ (.q3 i ψ <| hg ψ h1)).mp (asp ψ (.inl h1))
+    · apply asp (.fall i ψ)
+      rw [Set.mem_union]; right
+      rw [from_FOL_axiom] at h2 ⊢
+      obtain ⟨y, h3⟩ := h2
+      use .gen i y
+      unfold FOLAxioms.toFormula
+      rw [h3]
   | @mp x y _ _ p1 p2 => exact ((AX Γ (.q1 i x y)).mp p1).mp p2
 
 lemma all_elim (φ : Formula L) (i : Idx) : Γ ⊢ (∀i# φ) → φ :=
@@ -135,7 +141,7 @@ lemma all_comm (φ : Formula L) (i j : Idx) :
   have p5 := gen_rule _ φ i hi p4
   have p6 := gen_rule _ (∀i# φ) j hj p5
   have p7 := (deduction ∅ _ _).mp p6
-  have p8 := Proof.monotone (Set.empty_subset Γ) p7
+  have p8 := mono (Set.empty_subset Γ) p7
   (deduction Γ ..).mpr p8
 
 lemma impl_all_intro (i : Idx) {φ ψ : Formula L} (p : {φ} ⊢ ψ) : {∀i#φ} ⊢ ∀i#ψ :=
@@ -152,7 +158,7 @@ theorem loose_equiv (i : Idx) (t : Term L) (φ : Formula L) :
     ({φ.loose t i} ⊢ φ) ∧ ({φ} ⊢ φ.loose t i) := by
   open Formula Set in
   induction φ with
-  | atom | falsum => unfold loose; split_ands <;> exact asp _ (Set.mem_singleton _)
+  | atom | falsum => unfold loose; split_ands <;> exact AS (Set.mem_singleton _)
   | impl x y hx hy =>
     unfold loose
     repeat rw [Set.singleton_def, insert] at hx hy
@@ -160,14 +166,14 @@ theorem loose_equiv (i : Idx) (t : Term L) (φ : Formula L) :
     repeat rw [deduction] at hx hy
     split_ands
     · let ψ := loose t i x → loose t i y
-      have p1 := monotone (Set.empty_subset {ψ}) hx.right
-      have p2 := asp (α := FOLAxioms L) (Γ := {ψ}) ψ (Set.mem_singleton _)
-      have p3 := monotone (Set.empty_subset {ψ}) hy.left
+      have p1 := mono (Set.empty_subset {ψ}) hx.right
+      have p2 := AS (Set.mem_singleton ψ)
+      have p3 := mono (Set.empty_subset {ψ}) hy.left
       exact impl_trans (impl_trans p1 p2) p3
     · let ψ := x → y
-      have p1 := monotone (Set.empty_subset {ψ}) hx.left
-      have p2 := asp (α := FOLAxioms L) (Γ := {ψ}) ψ (Set.mem_singleton _)
-      have p3 := monotone (Set.empty_subset {ψ}) hy.right
+      have p1 := mono (Set.empty_subset {ψ}) hx.left
+      have p2 := AS (Set.mem_singleton ψ)
+      have p3 := mono (Set.empty_subset {ψ}) hy.right
       exact impl_trans (impl_trans p1 p2) p3
   | fall j ψ h =>
     rcases h with ⟨p1, p2⟩
@@ -191,7 +197,7 @@ theorem loose_equiv (i : Idx) (t : Term L) (φ : Formula L) :
       rw [h4] at p3
       replace p3 := (deduction ..).mpr p3
       conv at p1 => rw [Set.singleton_def]; dsimp [insert]; rw [deduction]
-      replace p1 := monotone (Set.empty_subset <| Set.insert (∀k#χ') ∅) p1
+      replace p1 := mono (Set.empty_subset <| Set.insert (∀k#χ') ∅) p1
       have h4 : j ∉ (∀k#χ').fvar := by
         unfold fvar
         rw [Set.mem_diff, Set.mem_singleton_iff, not_and, Decidable.not_not]
@@ -209,7 +215,7 @@ theorem loose_equiv (i : Idx) (t : Term L) (φ : Formula L) :
       replace hg := Or.resolve_right hg (Set.notMem_empty g)
       rw [hg]; exact h4
     · have p1 := impl_all_intro j p2
-      have p2 := Proof.AX ∅ (.q2 j (.var k) χ hj)
+      have p2 := AX ∅ (.q2 j (.var k) χ hj)
       have p3 := (deduction ..).mpr p2
       replace p3 := gen_rule _ _ k (by
         intro g hg
@@ -221,7 +227,7 @@ theorem loose_equiv (i : Idx) (t : Term L) (φ : Formula L) :
         exact hk <| Set.mem_of_mem_of_subset h (fvar_subset_vars χ)
         ) p3
       replace p3 := (deduction ..).mp p3
-      replace p3 := monotone (Set.empty_subset {fall j ψ}) p3
+      replace p3 := mono (Set.empty_subset {fall j ψ}) p3
       exact mp p3 p1
 end Proof
 end PrimaryLogic
