PrimaryLogic/FirstOrder/MaximalConsistent.lean
@@ -1,12 +1,14 @@
 import PrimaryLogic.Encoding
-import PrimaryLogic.Model
 import PrimaryLogic.FirstOrder.Theorem
 import PrimaryLogic.FirstOrder.Soundness
 
 namespace PrimaryLogic
 variable {LF LP : Type} {L : Lang LF LP} (Γ : Set (Formula L))
 
-def MaximalConsistent : Prop := Consistent (FOLAxioms L) Γ ∧ (∀ φ, φ ∈ Γ ∨ (¬φ) ∈ Γ)
+private abbrev InCon : Prop := Inconsistent (Γ ∪ FOLTheory)
+private abbrev Con : Prop := Consistent (Γ ∪ FOLTheory)
+
+def MaximalConsistent : Prop := Con Γ ∧ (∀ φ, φ ∈ Γ ∨ (¬φ) ∈ Γ)
 
 theorem maxConSet_iff (Γ : Set (Formula L)) (φ : Formula L) :
     MaximalConsistent Γ -> (φ ∈ Γ ↔ (Γ ⊢ φ)) := by
@@ -14,20 +16,17 @@ theorem maxConSet_iff (Γ : Set (Formula L)) (φ : Formula L) :
   open Proof in
   constructor
   · intro h
-    exact asp (α := FOLAxioms L) φ h
+    exact FOL.AS h
   · intro h
     have h' : (¬φ) ∉ Γ := by
       by_contra
-      have p1 := asp (α := FOLAxioms L) _ this
-      have p2 := mp (Γ := Γ) (α := FOLAxioms L) p1 h
+      have p1 := FOL.AS this
+      have p2 := mp p1 h
       exact m.left p2
     rcases m.right φ with h1 | h2
     · exact h1
     · exfalso; exact h' h2
-
-private abbrev InCon : Prop := Inconsistent (FOLAxioms L) Γ
-private abbrev Con : Prop := Consistent (FOLAxioms L) Γ
-
+/-
 lemma con_empty : Con (L := L) ∅ := by
   unfold Con Consistent Inconsistent
   by_contra
@@ -36,7 +35,7 @@ lemma con_empty : Con (L := L) ∅ := by
     fun x h => False.elim <| Set.notMem_empty x h
   unfold Formula.interpret at h2
   exact h2
-
+-/
 variable [Encodable LF] [Encodable LP] [DecidablePred (InCon (L := L))]
 
 def tryAdd (n : Nat) : Set (Formula L) :=
@@ -93,19 +92,22 @@ lemma maximalSet_compact (φ : Formula L) : (maxExpand Γ ⊢ φ) -> ∃ n : Nat
   intro p
   induction p with
   | asp ψ hg =>
-    rw [Set.mem_iUnion] at hg
-    obtain ⟨n, h⟩ := hg
-    use n
-    exact Proof.asp ψ h
-  | axm ax => use 0; exact Proof.axm ax
+    rw [Set.mem_union, Set.mem_iUnion] at hg
+    rcases hg with ⟨n, h⟩ | h
+    · use n
+      apply Proof.asp ψ
+      rw [Set.mem_union]
+      left; exact h
+    · use 0
+      exact FOL.axiom_proof h
   | @mp ψ χ p q hp hq =>
     obtain ⟨m, hm⟩ := hp
     obtain ⟨n, hn⟩ := hq
     use max m n
     have := expandAdd_monotone Γ m (max m n) (Nat.le_max_left m n)
-    have h1 := Proof.monotone this hm
+    have h1 := FOL.mono this hm
     have := expandAdd_monotone Γ n (max m n) (Nat.le_max_right m n)
-    have h2 := Proof.monotone this hn
+    have h2 := FOL.mono this hn
     exact Proof.mp h1 h2
 
 theorem Lindenbaum : Con Γ -> MaximalConsistent (maxExpand Γ) := by
